Refactoring

theories/ltl.v
@@ -1,73 +1,6 @@
-From iris.bi Require Import fixpoint_mono.
+From ltl Require Export trace.
 From iris.proofmode Require Import coq_tactics reduction spec_patterns.
 From iris.proofmode Require Export proofmode.
-
-Delimit Scope trace_scope with trace.
-
-CoInductive trace_aux (S L : Type) :=
-| tr_singl (s: S)
-| tr_cons (s: S) (ℓ: L) (r: trace_aux S L).
-
-Definition trace (S L : Type) := option $ trace_aux S L.
-
-Arguments tr_singl {_} {_} _.
-Arguments tr_cons {_} {_} _ _ _.
-
-Bind Scope trace_scope with trace.
-
-Arguments tr_singl {_} {_} _.
-Arguments tr_cons {_} {_} _ _ _%trace.
-Notation "⟨ ⟩" := (None) : trace_scope.
-Notation "⟨ s ⟩" := (Some (tr_singl s)) : trace_scope.
-Notation "s -[ ℓ ]->  r" := (Some (tr_cons s ℓ r)) (at level 33) : trace_scope.
-Open Scope trace.
-
-Section well_formed.
-  Context {S L : Type}.
-  Context (R : S → L → S → Prop).
-
-  Definition head_trace' (tr : trace_aux S L) : S * option L :=
-    match tr with
-    | tr_singl s => (s, None)
-    | tr_cons s ℓ tr => (s, Some ℓ)
-    end.
-
-  Definition head_trace : trace S L → option (S * option L) :=
-    fmap head_trace'.
-
-  Definition tail_trace' (tr : trace_aux S L) : option (trace_aux S L) :=
-    match tr with
-    | tr_singl s => None
-    | tr_cons s ℓ r => Some r
-    end.
-
-  Definition tail_trace : trace S L → trace S L :=
-    mbind tail_trace'.
-
-  CoInductive trace_maximal : trace S L → SProp :=
-  | trace_maximal_empty : trace_maximal None
-  | trace_maximal_singleton c :
-    (∀ oζ c', ¬ R c oζ c') → trace_maximal (Some $ tr_singl c)
-  | trace_maximal_cons c l tr c' :
-    fst <$> head_trace (Some tr) = Some c' →
-    R c l c' →
-    trace_maximal (Some tr) →
-    trace_maximal (Some $ tr_cons c l tr).
-
-End well_formed.
-
-Record wf_trace S L R := Trace {
-  tr_car : trace S L;
-  tr_wf : trace_maximal R tr_car;
-}.
-
-Arguments Trace {_ _ _} _ _.
-Arguments tr_car {_ _ _} _.
-Arguments tr_wf {_ _ _} _.
-Arguments trace_maximal_empty {_ _ _}.
-Arguments trace_maximal_singleton {_ _ _} _ _.
-
-Notation "tr @ tr_wf" := (Trace tr tr_wf) (at level 100).
 
 Definition tProp S L R := wf_trace S L R → Prop.
 
@@ -425,7 +358,7 @@ Section after.
 
 End after.
 
-Section ltl_always_constructor.
+Section ltl_constructors.
   Context {S L : Type}.
   Context {Rel : S → L → S → Prop}.
 
@@ -455,14 +388,15 @@ Section ltl_always_constructor.
   Definition ltl_always_unseal :
     @ltl_always = @ltl_always_def := seal_eq ltl_always_aux.
 
-End ltl_always_constructor.
+End ltl_constructors.
 
 Global Instance: Params (@ltl_next) 2 := {}.
+Global Instance: Params (@ltl_always) 2 := {}.
 
 Notation "○ P" := (ltl_next P%I) (at level 20, right associativity) : bi_scope.
 Notation "○^ n P" := (ltl_next_iter n P%I) (at level 20, n at level 9, P at level 20, format "○^ n  P") : bi_scope.
 
-Section ltl_always_lemmas.
+Section ltl_axioms.
   Context {S L : Type}.
   Context {Rel : S → L → S → Prop}.
 
@@ -609,6 +543,17 @@ Section ltl_always_lemmas.
     apply and_elim_r.
   Qed.
 
+  Lemma ltl_next_iter_mono_strong_pre n (P Q : tProp) :
+    ○^n (P → Q) ⊢ ○^n P → ○^n Q.
+  Proof.
+    induction n.
+    { done. }
+    simpl.
+    etrans; [|apply ltl_next_mono_strong].
+    apply ltl_next_mono_pre.
+    done.
+  Qed.
+
   (* K□ *)
   Lemma ltl_always_mono_strong_pre (P Q : tProp) :
     □ (P → Q) ⊢ □ P → □ Q.
@@ -619,13 +564,8 @@ Section ltl_always_lemmas.
     etrans; [apply and_intro|].
     { etrans; [apply and_elim_l|]. apply (forall_elim n). }
     { etrans; [apply and_elim_r|]. apply (forall_elim n). }
-    induction n.
-    { simpl. apply impl_elim_l'. done. }
-    simpl.
     apply impl_elim_l'.
-    etrans; [|apply ltl_next_mono_strong].
-    apply ltl_next_mono_pre.
-    apply impl_intro_r. done.
+    apply ltl_next_iter_mono_strong_pre.
   Qed.
 
   Lemma ltl_next_forall_1 {A} (P : A → tProp) :
@@ -640,6 +580,34 @@ Section ltl_always_lemmas.
     - simplify_eq. intros x. specialize (Hnext x).
       simplify_eq. done.
   Qed.
+
+End ltl_axioms.
+
+Section ltl_lemmas.
+  Context {S L : Type}.
+  Context {Rel : S → L → S → Prop}.
+
+  Notation tProp := (tProp S L Rel).
+  Implicit Type P Q : tProp.
+
+  (** The notations below are implicitly local due to the section, so we do not
+  mind the overlap with the general BI notations. *)
+  Notation "P ⊢ Q" := (ltl_entails P Q).
+  Notation "'True'" := (ltl_pure True) : bi_scope.
+  Notation "'False'" := (ltl_pure False) : bi_scope.
+  Notation "'⌜' φ '⌝'" := (ltl_pure φ%type%stdpp) : bi_scope.
+  Infix "∧" := ltl_and : bi_scope.
+  Infix "∨" := ltl_or : bi_scope.
+  Infix "→" := ltl_impl : bi_scope.
+  Notation "∀ x .. y , P" :=
+    (ltl_forall (λ x, .. (ltl_forall (λ y, P%I)) ..)) : bi_scope.
+  Notation "∃ x .. y , P" :=
+    (ltl_exist (λ x, .. (ltl_exist (λ y, P%I)) ..)) : bi_scope.
+  Notation "▷ P" := (ltl_later P) : bi_scope.
+  Notation "x ≡ y" := (ltl_internal_eq x y) : bi_scope.
+  Notation "□ P" := (ltl_always P) : bi_scope.
+
+  (** Derived constructs *)
 
   Lemma ltl_always_unfold_pre_1 (P : tProp) :
     □ P ⊢ P ∧ ○ □ P.
@@ -675,7 +643,6 @@ Section ltl_always_lemmas.
     apply impl_intro_r.
     apply forall_intro=> n.
     apply impl_elim_l'.
-    (* etrans; [apply (forall_elim n)|]. *)
     induction n=> /=.
     { apply impl_intro_r, and_elim_r. }
     etrans; [apply ltl_always_unfold_pre_1|].
@@ -691,8 +658,6 @@ Section ltl_always_lemmas.
     apply ltl_next_mono_pre.
     done.
   Qed.
-
-  (** Derived constructs *)
 
   Lemma ltl_always_emp :
     True ⊢ (□ True) : tProp.
@@ -755,9 +720,9 @@ Section ltl_always_lemmas.
     - apply and_elim_r.
   Qed.
 
-End ltl_always_lemmas.
+End ltl_lemmas.
 
-Section ltl.
+Section ltl_bi.
   Context {S L : Type}.
   Context {Rel : S → L → S → Prop}.
 
@@ -878,7 +843,7 @@ Section ltl.
       rewrite ltl_or_unseal. right. rewrite ltl_impl_unseal. intros HP. done.
   Qed.
 
-End ltl.
+End ltl_bi.
 
 Canonical Structure ltlI {S L : Type} {Rel} : bi :=
   {| bi_ofe_mixin := ofe_mixin_of (tProp S L Rel);
@@ -886,7 +851,7 @@ Canonical Structure ltlI {S L : Type} {Rel} : bi :=
     bi_bi_persistently_mixin := ltl_bi_persistently_mixin;
     bi_bi_later_mixin := ltl_bi_later_mixin |}.
 
-Section ltl.
+Section ltl_bi_typeclasses.
   Context {S L : Type}.
   Context {Rel : S → L → S → Prop}.
 
@@ -898,7 +863,7 @@ Section ltl.
   (* Also add this to the global hint database, otherwise [eauto] won't work for
 many lemmas that have [BiAffine] as a premise. *)
 
-End ltl.
+End ltl_bi_typeclasses.
 
 Global Hint Immediate ltl_affine : core.
 
@@ -941,22 +906,15 @@ Section restate.
 
   Definition ltl_unseal :=
     (ltl_emp_unseal, ltl_pure_unseal, ltl_and_unseal, ltl_or_unseal,
-    ltl_impl_unseal, ltl_forall_unseal, ltl_exist_unseal,
-    ltl_sep_unseal, ltl_wand_unseal,
-    ltl_persistently_unseal, ltl_later_unseal).
+     ltl_impl_unseal, ltl_forall_unseal, ltl_exist_unseal,
+     ltl_sep_unseal, ltl_wand_unseal,
+     ltl_persistently_unseal, ltl_later_unseal).
 End restate.
 
 (** The final unseal tactic that also unfolds the BI layer. *)
 Ltac unseal := rewrite !ltl_unseal /=.
 End tProp.
 
-(* Global Instance ltl_next_proper {S L Rel} : Proper ((≡) ==> (≡)) (@ltl_next S L Rel). *)
-(* Proof. Admitted. *)
-(*   rewrite ltl_next_unseal. *)
-(*   constructor. *)
-(*   intros. *)
-(*   constructor; inversion 1; simplify_eq; econstructor; by apply H. *)
-(* Qed. *)
 Global Instance ltl_next_mono' {S L Rel} :
   Proper ((⊢) ==> (⊢)) (@ltl_next S L Rel).
 Proof.
@@ -971,7 +929,7 @@ Proof.
   constructor. intros. by apply H.
 Qed.
 
-Section ltl_lemmas.
+Section ltl_axioms.
   Context {S L : Type}.
   Context {Rel : S → L → S → Prop}.
 
@@ -1020,6 +978,14 @@ Section ltl_lemmas.
   Lemma ltl_dup (P : tProp) : P ⊢ P ∧ P.
   Proof. iIntros "H". iFrame. Qed.
 
+  Lemma ltl_sep_and (P Q : tProp) :
+    P ∗ Q ⊣⊢ P ∧ Q.
+  Proof. done. Qed.
+
+  Lemma ltl_wand_impl (P Q : tProp) :
+    (P -∗ Q) ⊣⊢ (P → Q).
+  Proof. done. Qed.
+
   (** AXIOMS *)
 
   (** ltl_next lemmas *)
@@ -1028,14 +994,6 @@ Section ltl_lemmas.
   Lemma ltl_next_taut (P : tProp) :
     (⊢ P) → (⊢ ○ P).
   Proof. apply ltl_next_taut'. Qed.
-  (* K○ *)
-  (* Lemma ltl_next_mono_strong (P Q : tProp) : *)
-  (*   ○ (P → Q) ⊢ ○ P → ○ Q. *)
-  (* Proof. *)
-  (*   constructor. ltl_unseal. unseal. *)
-  (*   intros [tr wf] HPQ HP. *)
-  (*   inversion HP; inversion HPQ; simplify_eq; econstructor; try naive_solver. *)
-  (* Qed. *)
 
   (* A2 *)
   Lemma ltl_next_not (P : tProp) :
@@ -1062,17 +1020,43 @@ Section ltl_lemmas.
     eexists _. apply H.
   Qed.
 
-End ltl_lemmas.
+  (** Next Iter *)
 
-Section ltl_derived_rules.
-  Context {S L : Type}.
-  Context {Rel : S → L → S → Prop}.
+  Lemma ltl_next_iter_mono_strong n (P Q : tProp) :
+    ○^n (P → Q) ⊢ ○^n P → ○^n Q.
+  Proof. apply ltl_next_iter_mono_strong_pre. Qed.
 
-  Notation tProp := (tProp S L Rel).
+  Lemma ltl_next_iter_taut n (P : tProp) :
+    (⊢ P) → (⊢ ○^n P).
+  Proof.
+    intros HP.
+    induction n; [done|].
+    simpl. apply ltl_next_taut. done.
+  Qed.
 
-  (** DERIVED RULES *)
+  Lemma ltl_next_iter_mono n (P Q : tProp) :
+    (P ⊢ Q) → (○^n P ⊢ ○^n Q).
+  Proof.
+    iIntros (HPQ) "HPQ". iRevert "HPQ". iApply ltl_next_iter_mono_strong.
+    iApply ltl_next_iter_taut. iIntros "HP". by iApply HPQ.
+  Qed.
 
-  (* Always *)
+  Lemma ltl_iter_forall (P:tProp) :
+    (∀ n, ○^n P)%I ⊢ ○ (∀ n, ○^n P).
+  Proof.
+    iIntros "HP". rewrite -ltl_next_forall_1. iIntros (n).
+    iSpecialize ("HP" $! (Datatypes.S n)). done.
+  Qed.
+
+  Global Instance ltl_next_iter_proper n : Proper ((≡) ==> (≡)) (@ltl_next_iter S L Rel n).
+  Proof.
+    intros P Q Heq.
+    induction n.
+    { simpl. done. } 
+    simpl. f_equiv. done.
+  Qed.
+
+  (** Restating ltl_always lemmas *)
 
   Lemma ltl_always_unfold (P : tProp) :
     □ P ⊣⊢ P ∧ ○ □ P.
@@ -1086,28 +1070,34 @@ Section ltl_derived_rules.
     □ (P → ○ P) ⊢ P → □ P.
   Proof. rewrite !bi_intuitionistically_unseal. apply ltl_always_intro_pre. Qed.
 
-  (* Lemma ltl_always_coind (P : tProp) : *)
-  (*   □ (P → ○ P) ⊢ P → □ P. *)
-  (* Proof. rewrite !bi_intuitionistically_unseal. apply ltl_always_intro_pre. Qed. *)
-
   Lemma ltl_always_elim (P : tProp) :
     □ P ⊢ P.
   Proof. rewrite ltl_always_unfold. iIntros "[$ _]". Qed.
+
+  Lemma ltl_next_mono (P Q : tProp) :
+    (P ⊢ Q) → (○ P ⊢ ○ Q).
+  Proof. apply ltl_next_mono_pre. Qed.
 
   (* Actual A1 / K□ *)
   Lemma ltl_always_mono_strong (P Q : tProp) :
     □ (P → Q) ⊢ □ P → □ Q.
   Proof.  rewrite !bi_intuitionistically_unseal. apply ltl_always_mono_strong_pre. Qed.
 
+End ltl_axioms.
+
+Section ltl_derived_rules.
+  Context {S L : Type}.
+  Context {Rel : S → L → S → Prop}.
+
+  Notation tProp := (tProp S L Rel).
+
+  (** DERIVED RULES *)
+
   (* Next *)
 
   Lemma ltl_next_emp :
     True ⊢ ○ True : tProp.
-  Proof. iIntros "_". by iApply ltl_next_taut. Qed.
-
-  Lemma ltl_next_mono (P Q : tProp) :
-    (P ⊢ Q) → (○ P ⊢ ○ Q).
-  Proof. apply ltl_next_mono_pre. Qed.
+  Proof. by apply ltl_next_taut. Qed.
 
   Lemma ltl_false_next :
     ○ False ⊢ False : tProp.
@@ -1193,11 +1183,40 @@ Section ltl_derived_rules.
     (□ P ∧ ○ Q) ⊢ (○ (Q ∧ □ P)).
   Proof. by rewrite bi.and_comm {1}ltl_always_next ltl_next_and. Qed.
 
-  (** Proofmode stuff *)
+  Lemma ltl_always_unseal' (P:tProp) : 
+    (□ P)%I ≡ (∀ n, ○^n P)%I.
+  Proof.   
+    rewrite !bi_intuitionistically_unseal.
+    rewrite ltl_always_unseal.
+    done.
+  Qed.
 
-  Lemma ltl_sep_and (P Q : tProp) :
-    P ∗ Q ⊣⊢ P ∧ Q.
-  Proof. done. Qed.
+  Lemma ltl_always_coind (P Q : tProp) :
+    □ (P → (Q ∧ ○ (P ∨ □ Q))) ⊢ P → □ Q.
+  Proof.
+    rewrite !ltl_always_unseal'.
+    iIntros "H".
+    iEval (rewrite !ltl_always_unseal').
+    iIntros "HP" (n).
+    iInduction n as [|n IHn] forall (P Q).
+    { simpl. iSpecialize ("H" $! 0). iDestruct ("H" with "HP") as "[HQ _]". done. }
+    replace (Datatypes.S n) with (1 + n) by lia.
+    rewrite !ltl_next_iter_sum.
+    iDestruct (ltl_dup with "H") as "[H H']".
+    iSpecialize ("H" $! 0). simpl.
+    iDestruct ("H" with "HP") as "[HQ H]".
+    rewrite ltl_iter_forall.
+    iCombine "H H'" as "H". rewrite ltl_sep_and ltl_next_and.
+    iRevert "H". rewrite ltl_wand_impl. iApply ltl_next_mono_strong.
+    rewrite ltl_wand_impl.
+    iApply ltl_always_elim. iApply ltl_always_next_comm. iApply ltl_always_next.
+    iIntros "!> [H H']".
+    iDestruct "H" as "[HP|HQ]"; last first.
+    { iDestruct (ltl_always_unseal' with "HQ") as "HQ". iApply "HQ". }
+    iApply ("IHn" with "[H'] HP").
+    iIntros (m).
+    iApply "H'".
+  Qed.
 
 End ltl_derived_rules.
 
@@ -1206,8 +1225,6 @@ Section ltl_proofmode.
   Context {Rel : S → L → S → Prop}.
 
   Notation tProp := (tProp S L Rel).
-
-  Import tProp.
 
   (* Proofmode support for next modality *)
 
@@ -1321,596 +1338,3 @@ Section ltl_proofmode.
   Qed.
 
 End ltl_proofmode.
-
-Section ltl_derived_constructs.
-  Context {S L : Type}.
-  Context {Rel : S → L → S → Prop}.
-
-  Notation tProp := (tProp S L Rel).
-
-  (* LTL Next Iter *)
-  Lemma ltl_next_iter_mono n (P Q : tProp) :
-    ○^n (P → Q) ⊢ ○^n P → ○^n Q.
-  Proof.
-    iIntros "HPQ HP".
-    iInduction n as [|n IHn].
-    { by iApply "HPQ". }
-    simpl in *.
-    iModIntro.
-    iApply ("IHn" with "HPQ HP").
-  Qed.
-
-  Global Instance ltl_next_iter_proper n : Proper ((≡) ==> (≡)) (@ltl_next_iter S L Rel n).
-  Proof.
-    intros P Q Heq.
-    induction n.
-    { simpl. done. } 
-    simpl. f_equiv. done.
-  Qed.
-
-  Lemma ltl_iter_forall (P:tProp) :
-    (∀ n, ○^n P)%I ⊢ ○ (∀ n, ○^n P).
-  Proof.
-    iIntros "HP". rewrite -ltl_next_forall_1. iIntros (n).
-    iSpecialize ("HP" $! (Datatypes.S n)). done.
-  Qed.
-
-  Lemma ltl_always_unseal' (P:tProp) : 
-    (□ P)%I ≡ (∀ n, ○^n P)%I.
-  Proof.   
-    rewrite !bi_intuitionistically_unseal.
-    rewrite ltl_always_unseal.
-    done.
-  Qed.
-
-  Lemma ltl_always_coind (P Q : tProp) :
-    □ (P → (Q ∧ ○ (P ∨ □ Q))) ⊢ P → □ Q.
-  Proof.
-    rewrite !ltl_always_unseal'.
-    iIntros "H".
-    iEval (rewrite !ltl_always_unseal').
-    iIntros "HP" (n).
-    iInduction n as [|n IHn] forall (P Q).
-    { simpl. iSpecialize ("H" $! 0). iDestruct ("H" with "HP") as "[HQ _]". done. }
-    replace (Datatypes.S n) with (1 + n) by lia.
-    rewrite !ltl_next_iter_sum.
-    iDestruct (ltl_dup with "H") as "[H H']".
-    iSpecialize ("H" $! 0). simpl.
-    iDestruct ("H" with "HP") as "[HQ H]".
-    rewrite ltl_iter_forall.
-    iModIntro.
-    iDestruct "H" as "[HP|HQ]"; last first.
-    { rewrite {2}ltl_always_unseal'. iApply "HQ". }
-    iApply ("IHn" with "[H'] HP").
-    iIntros (m).
-    iApply "H'".
-  Qed.
-
-  Lemma ltl_always_intro_alt (P : tProp) :
-    □ (P → ○ P) ⊢ P → □ P.
-  Proof.
-    iIntros "#IH HP". iApply (ltl_always_coind with "[] HP").
-    iIntros "!> HP". iSplit; [done|]. iDestruct ("IH" with "HP") as "HP".
-    iModIntro. iLeft. done.
-  Qed.
-
-  (* Until *)
-  Definition ltl_until_F (P Q : tProp) : (() → tProp) → (() → tProp) :=
-    (λ (X : unit → tProp) _, Q ∨ (P ∧ ○ (X ())))%I.
-
-  Instance ltl_until_F_mono P Q : BiMonoPred (ltl_until_F P Q).
-  Proof.
-    constructor.
-    - intros. iIntros "#H" (x) "HF".
-      rewrite /ltl_until_F.
-      iDestruct "HF" as "[HQ|[HP HF]]"; [by iLeft|].
-      iRight. iFrame.
-      iModIntro. by iApply "H".
-    - intros. apply _.
-  Qed.
-
-  Definition ltl_until_def (P Q : tProp) : tProp :=
-    bi_least_fixpoint (ltl_until_F P Q)%I ().
-  Definition ltl_until_aux : seal (@ltl_until_def).
-  Proof. by eexists. Qed.
-  Definition ltl_until := unseal ltl_until_aux.
-  Definition ltl_until_unseal :
-    @ltl_until = @ltl_until_def := seal_eq ltl_until_aux.
-
-  Notation "P ∪ Q" := (ltl_until P Q%I) : bi_scope.
-  Notation "◊ P" := (ltl_until True P%I) (at level 20, right associativity) : bi_scope.
-
-  Lemma ltl_until_unfold (P Q : tProp) :
-    (P ∪ Q)%I ≡ (Q ∨ P ∧ ○ (P ∪ Q))%I.
-  Proof. rewrite ltl_until_unseal. by rewrite /ltl_until_def {1}least_fixpoint_unfold. Qed.
-
-  Lemma ltl_until_intro (P Q : tProp) :
-    Q ∨ P ∧ ○ (P ∪ Q) ⊢ P ∪ Q.
-  Proof. rewrite {2}ltl_until_unfold. done. Qed.
-
-  Lemma ltl_until_ind_strong (P Q R : tProp) :
-    □ (Q ∨ (P ∧ ○ (P ∪ Q) ∧ ○ R) → R) ⊢
-    P ∪ Q → R.
-  Proof.
-    iIntros "#IH HPQ".
-    rewrite ltl_until_unseal.
-    iApply (least_fixpoint_ind with "[] HPQ").
-    iIntros "!>" (?) "[Q|[HP HR]]".
-    { iApply "IH". by eauto. }
-    iApply "IH". iRight. iFrame.
-    iSplit.
-    - iModIntro. iDestruct "HR" as "[_ $]".
-    - iModIntro. iDestruct "HR" as "[$ _]".
-  Qed.
-
-  Lemma ltl_until_ind (P Q R : tProp) :
-    (Q ∨ (P ∧ ○ (P ∪ Q) ∧ ○ R) ⊢ R) →
-    (P ∪ Q ⊢ R).
-  Proof.
-    intros IH.
-    iApply ltl_until_ind_strong. iIntros "!> H". iApply IH. done.
-  Qed.
-
-  Lemma ltl_until_intro_now (P Q : tProp) :
-    Q ⊢ P ∪ Q.
-  Proof. rewrite -ltl_until_intro. apply bi.or_intro_l. Qed.
-
-  Lemma ltl_until_intro_next (P Q : tProp) :
-    P ∧ ○ (P ∪ Q) ⊢ P ∪ Q.
-  Proof. rewrite -{2}ltl_until_intro. apply bi.or_intro_r. Qed.
-
-  Lemma ltl_until_mono_strong P1 P2 Q1 Q2 :
-    □ (P1 → P2) ⊢ □ (Q1 → Q2) →
-    P1 ∪ Q1 → P2 ∪ Q2.
-  Proof.
-    iIntros "#HP #HQ HPQ".
-    iApply (ltl_until_ind_strong with "[] HPQ").
-    iModIntro.
-    iDestruct 1 as "[H|H]".
-    { rewrite ltl_until_unfold. iLeft. by iApply "HQ". }
-    iEval (rewrite ltl_until_unfold). iRight.
-    iDestruct "H" as "[H IH]".
-    iSplit.
-    - by iApply "HP".
-    - iDestruct "IH" as "[_ $]".
-  Qed.
-
-  Lemma ltl_until_mono P1 P2 Q1 Q2 :
-    (P1 ⊢ P2) → (Q1 ⊢ Q2) →
-    P1 ∪ Q1 ⊢ P2 ∪ Q2.
-  Proof.
-    intros HP HQ.
-    iApply ltl_until_mono_strong.
-    iApply HP.
-    iApply HQ.
-  Qed.
-
-  Lemma ltl_until_and (P Q1 Q2 : tProp) :
-    (P ∪ (Q1 ∧ Q2)) ⊢ (P ∪ Q1) ∧ (P ∪ Q2).
-  Proof.
-    rewrite ltl_until_unfold.
-    iIntros "[H|H]".
-    { iDestruct "H" as "[H1 H2]".
-      rewrite (ltl_until_unfold _ Q1).
-      rewrite (ltl_until_unfold _ Q2).
-      iSplit; by iLeft. }
-    iSplit.
-    - iEval (rewrite ltl_until_unfold).
-      iRight. iDestruct "H" as "[$ H]".
-      iModIntro. iApply (ltl_until_mono_strong with "[] [] H").
-      + eauto.
-      + iIntros "!>[$ _]".
-    - iEval (rewrite ltl_until_unfold).
-      iRight. iDestruct "H" as "[$ H]".
-      iModIntro. iApply (ltl_until_mono_strong with "[] [] H").
-      + eauto.
-      + iIntros "!>[_ $]".
-  Qed.
-
-  Lemma ltl_until_always_combine (P Q R : tProp) :
-    (□ P ∧ Q ∪ R) ⊢ (((Q ∧ □ P) ∪ (R ∧ □ P))).
-  Proof.
-    iIntros "[#HP HQ]".
-    iApply (ltl_until_ind_strong with "[] HQ").
-    iIntros "!> [HQ|H]".
-    { iApply ltl_until_intro_now. iFrame "#∗". }
-    iEval (rewrite -ltl_until_intro_next).
-    iDestruct "H" as "[$ H]".
-    iSplit; [done|].
-    iModIntro.
-    iDestruct "H" as "[_ $]".
-  Qed.
-
-  Lemma ltl_until_next_comm (P Q : tProp) :
-    (○ P ∪ ○ Q) ⊣⊢ ○ (P ∪ Q).
-  Proof.
-    iSplit.
-    - iApply ltl_until_ind_strong.
-      iIntros "!>H".
-      iDestruct "H" as "[HQ|H]".
-      + iModIntro. rewrite ltl_until_unfold. by iLeft.
-      + iModIntro. iEval (rewrite ltl_until_unfold). iRight.
-        iDestruct "H" as "[$ [HP HQ]]". iModIntro. done.
-    - iIntros "H".
-      iEval (rewrite ltl_until_unfold).
-      rewrite ltl_next_and.
-      iEval (rewrite (ltl_next_or Q)).
-      iModIntro.
-      iApply (ltl_until_ind_strong with "[] H").
-      iIntros "!>H".
-      iDestruct "H" as "[H|H]".
-      { iLeft. done. }
-      iRight.
-      iDestruct "H" as "[$ [_ H]]".
-      rewrite {2}ltl_until_unfold.
-      rewrite ltl_next_and ltl_next_or.
-      iModIntro.
-      iDestruct "H" as "[H|H]".
-      { iLeft. done. }
-      iRight.
-      done.
-  Qed.
-
-  Lemma ltl_until_idemp (P Q : tProp) :
-    (P ∪ (P ∪ Q)) ⊣⊢ (P ∪ Q).
-  Proof.
-    iSplit.
-    - iApply ltl_until_ind_strong.
-      iIntros "!> [H|(?&?&?)]".
-      { done. }
-      iEval (rewrite ltl_until_unfold). iRight. iFrame.
-    - iApply ltl_until_ind_strong.
-      iIntros "!> [H|(?&?&?)]".
-      { rewrite ltl_until_unfold. iLeft. rewrite ltl_until_unfold. iLeft. done. }
-      iEval (rewrite ltl_until_unfold). iRight. iFrame.
-  Qed.
-
-  Lemma ltl_until_and_r' (P1 P2 Q1 Q2 : tProp) :
-    P1 ∪ Q1 ∧ P2 ∪ Q2 ⊢ (P1 ∧ P2) ∪ ((Q1 ∧ P2 ∪ Q2) ∨ (P1 ∪ Q1 ∧ Q2)).
-  Proof.
-    iIntros "[H1 H2]".
-    iRevert "H2".
-    iApply (ltl_until_ind_strong with "[] H1").
-    iIntros "!> H1 H2".
-    rewrite {3}(ltl_until_unfold P2 Q2).
-    iDestruct "H1" as "[HQ1|(HP1&HPQ1&IH)]".
-    { iDestruct "H2" as "[HQ2|[HP2 HPQ2]]".
-      { iEval (rewrite ltl_until_unfold). iLeft.
-        iEval (rewrite ltl_until_unfold). iFrame. }
-      { iEval (rewrite ltl_until_unfold). iLeft. iLeft. iFrame.
-        iEval (rewrite ltl_until_unfold). iRight. iFrame. }
-    }
-    iDestruct "H2" as "[HQ2|[HP2 HPQ2]]".
-    { iEval (rewrite ltl_until_unfold). iLeft.
-      iEval (rewrite ltl_until_unfold). iRight.
-      iEval (rewrite ltl_until_unfold). iFrame. iRight. iFrame. }
-    iEval (rewrite ltl_until_unfold). iRight.
-    iFrame. iModIntro.
-    by iApply "IH".
-  Qed.
-
-  Lemma ltl_until_or (P Q1 Q2 : tProp) :
-    P ∪ (Q1 ∨ Q2) ⊢ P ∪ Q1 ∨ P ∪ Q2.
-  Proof.
-    iApply ltl_until_ind_strong.
-    iIntros "!> [HQ|HP]".
-    { iDestruct "HQ" as "[HQ1|HQ2]".
-      - iLeft. by rewrite -ltl_until_intro_now.
-      - iRight. by rewrite -ltl_until_intro_now.
-    }
-    iDestruct "HP" as "(HP&HPQ&IH)".
-    rewrite -!ltl_until_next_comm.
-    rewrite {1}(ltl_next_or_2 (P ∪ Q1)).
-    iDestruct "IH" as "[IH|IH]".
-    - iLeft. iEval (rewrite ltl_until_unfold).
-      iRight. iFrame.
-    - iRight. iEval (rewrite ltl_until_unfold).
-      iRight. iFrame.
-  Qed.
-
-  Lemma ltl_until_and_r (P1 P2 Q1 Q2 : tProp) :
-    P1 ∪ Q1 ∧ P2 ∪ Q2 ⊢ ((P1 ∧ P2) ∪ (Q1 ∧ (P2 ∪ Q2))) ∨ ((P1 ∧ P2) ∪ (P1 ∪ Q1 ∧ Q2)).
-  Proof. rewrite -ltl_until_or. apply ltl_until_and_r'. Qed.
-
-  Global Instance ltl_until_proper : Proper ((≡) ==> (≡) ==> (≡)) (ltl_until).
-  Proof.
-    constructor.
-    intros. split.
-    - apply ltl_until_mono; [by rewrite H|by rewrite H0].
-    - apply ltl_until_mono; [by rewrite H|by rewrite H0].
-  Qed.
-  Global Instance ltl_until_mono' :
-    Proper ((⊢) ==> (⊢) ==> (⊢)) (ltl_until).
-  Proof.
-    constructor.
-    intros ?. apply ltl_until_mono; [by rewrite H|by rewrite H0].
-  Qed.
-  Global Instance ltl_until_flip_mono' :
-    Proper (flip (⊢) ==> flip (⊢) ==> flip (⊢)) (ltl_until).
-  Proof.
-    constructor.
-    intros ?. apply ltl_until_mono; [by rewrite H|by rewrite H0].
-  Qed.
-
-  Global Instance ltl_until_combine (P1 P2 Q1 Q2 : tProp) :
-    CombineSepAs (P1 ∪ Q1) (P2 ∪ Q2)
-      (((P1 ∧ P2) ∪ (Q1 ∧ (P2 ∪ Q2))) ∨ ((P1 ∧ P2) ∪ (P1 ∪ Q1 ∧ Q2))) | 1.
-  Proof. rewrite /CombineSepAs. apply ltl_until_and_r. Qed.
-
-  Lemma ltl_eventually_intro (P : tProp) :
-    P ∨ ○ ◊ P ⊢ ◊ P.
-  Proof.
-    rewrite -{2}(ltl_until_intro True P).
-    iIntros "[HP|HP]".
-    { by iLeft. }
-    iRight. by iFrame.
-  Qed.
-
-  Lemma ltl_eventually_intro_now (P : tProp) :
-    P ⊢ ◊ P.
-  Proof. rewrite -ltl_until_intro. apply bi.or_intro_l. Qed.
-
-  Lemma ltl_eventually_intro_next (P : tProp) :
-    (○ P) ⊢ (◊ P).
-  Proof. rewrite -ltl_eventually_intro.
-         etrans; [|apply bi.or_intro_r]. apply ltl_next_mono.
-         apply ltl_eventually_intro_now.
-  Qed.
-
-  Lemma ltl_eventually_mono_strong (P Q : tProp) :
-    □ (P → Q) ⊢ ◊P → ◊Q.
-  Proof. by iApply ltl_until_mono_strong. Qed.
-
-  Lemma ltl_eventually_mono (P Q : tProp) :
-    (P ⊢ Q) → (◊P) ⊢ (◊Q).
-  Proof. by apply ltl_until_mono. Qed.
-
-  Lemma ltl_eventually_and (P Q : tProp) :
-    (◊ (P ∧ Q)) ⊢ (◊ P) ∧ (◊ Q).
-  Proof. by rewrite -ltl_until_and. Qed.
-
-  Lemma ltl_eventually_next_comm (P : tProp) :
-    (◊ ○ P) ⊣⊢ (○ ◊ P).
-  Proof.
-    rewrite -ltl_until_next_comm.
-    apply bi.equiv_entails_2.
-    - apply ltl_until_mono; [|done]. by apply ltl_next_emp.
-    - apply ltl_until_mono; [|done]. eauto.
-  Qed.
-
-  Lemma ltl_eventually_idemp (P : tProp) :
-    (◊◊P) ⊣⊢ (◊P).
-  Proof. apply ltl_until_idemp. Qed.
-
-  Lemma ltl_eventually_next (P : tProp) :
-    (◊ ○ P) ⊢ (◊ P).
-  Proof.
-    rewrite <-(ltl_eventually_idemp P).
-    apply ltl_eventually_mono.
-    apply ltl_eventually_intro_next.
-  Qed.
-
-  Lemma ltl_next_eventually (P : tProp) :
-    (○ ◊ P) ⊢ (◊ P).
-  Proof. rewrite -{2}ltl_eventually_next ltl_eventually_next_comm. done. Qed.
-
-  Lemma ltl_until_eventually_equiv (P : tProp) :
-    (True ∪ P) ⊣⊢ (◊ P).
-  Proof. done. Qed.
-
-  Lemma ltl_until_eventually (P Q : tProp) :
-    (P ∪ Q) ⊢ (◊ Q).
-  Proof. apply ltl_until_mono; by eauto. Qed.
-
-  Lemma ltl_eventually_ind_strong (P Q : tProp) :
-    (□ (P ∨ ○ ◊ P ∧ ○ Q → Q)) ⊢ ◊ P → Q.
-  Proof.
-    iIntros "#H". iApply ltl_until_ind_strong.
-    iModIntro. iIntros "[HP|HP]".
-    { iApply "H". iLeft. done. }
-    iApply "H". iRight. iDestruct "HP" as "[_ $]".
-  Qed.
-
-  Lemma ltl_eventually_ind (P Q : tProp) :
-    (P ⊢ Q) →
-    ((○ ◊ P) ∧ ○ Q ⊢ Q) →
-    ◊ P ⊢ Q.
-  Proof.
-    intros H1 H2.
-    iApply ltl_eventually_ind_strong.
-    iDestruct H1 as "#H1".
-    iDestruct H2 as "#H2".
-    iModIntro. iIntros "[HP|HP]"; [by iApply "H1"|by iApply "H2"].
-  Qed.
-
-  Lemma ltl_always_eventually (P : tProp) :
-    □ P ⊢ ◊ P.
-  Proof. rewrite -ltl_eventually_intro_now. eauto. Qed.
-
-  Lemma ltl_eventually_always_combine (P Q : tProp) :
-    (□ P ∧ ◊Q) ⊢ (◊ (Q ∧ □ P)).
-  Proof.
-    iIntros "[#HP HQ]".
-    iApply (ltl_eventually_ind_strong with "[] HQ").
-    iIntros "!> [HQ|H]".
-    { iApply ltl_eventually_intro_now. iFrame "#∗". }
-    iEval (rewrite -ltl_eventually_idemp).
-    iEval (rewrite -ltl_eventually_intro_next).
-    iModIntro.
-    iDestruct "H" as "[_ $]".
-  Qed.
-
-  Lemma ltl_not_eventually_always_not (P : tProp) :
-    ¬ ◊ P ⊢ □ (¬ P).
-  Proof.
-    iIntros "H".
-    iAssert (□ ((¬ ◊ P) ∧ (¬ P)))%I with "[H]" as "#[H1 H2]"; last first.
-    { iApply ltl_always_intro; last first.
-      { done. }
-      iIntros "!> H !>". iFrame "#". }
-    iApply ltl_always_intro; last first.
-    { iSplit.
-      - done.
-      - iIntros "HP". iApply "H". rewrite -ltl_eventually_intro_now. done. }
-    iIntros "!> [H1 H2]".
-    rewrite -ltl_next_and.
-    iSplit.
-    - rewrite -ltl_next_not. iIntros "H". iApply "H1". rewrite ltl_next_eventually. done.
-    - rewrite -ltl_next_not. iIntros "H". iApply "H1". rewrite -ltl_next_eventually. iModIntro. rewrite -ltl_eventually_intro_now. done.
-  Qed.
-
-  Global Instance into_and_eventually (P Q1 Q2 : tProp) :
-    IntoAnd false P Q1 Q2 →
-    IntoAnd false (◊ P)%I (◊ Q1)%I (◊ Q2)%I.
-  Proof.
-    rewrite /IntoAnd. simpl.
-    intros HPQ.
-    rewrite -ltl_eventually_and.
-    by eapply ltl_eventually_mono.
-  Qed.
-
-  Global Instance into_sep_eventually (P Q1 Q2 : tProp) :
-    IntoSep P Q1 Q2 →
-    IntoSep (◊ P)%I (◊ Q1)%I (◊ Q2)%I.
-  Proof.
-    rewrite /IntoSep.
-    simpl.
-    rewrite !bi_sep_and.
-    intros HPQ.
-    rewrite -ltl_eventually_and.
-    by eapply ltl_eventually_mono.
-  Qed.
-
-  Global Instance into_next_eventually (P Q : tProp) :
-    IntoNext false P Q →
-    IntoNext false (◊ P) (◊ Q).
-  Proof.
-    rewrite /IntoNext. intros HPQ.
-    rewrite -ltl_eventually_next_comm.
-    eapply ltl_eventually_mono.
-    specialize HPQ. simpl in HPQ.
-    done.
-  Qed.
-
-  Lemma ltl_eventually_and_r (P Q : tProp) :
-    ◊ P ∧ ◊ Q ⊢ ◊ (P ∧ ◊ Q) ∨ ◊ (◊ P ∧ Q).
-  Proof. by rewrite ltl_until_and_r right_id. Qed.
-
-  Global Instance ltl_eventually_combine (P Q : tProp) :
-    CombineSepAs (◊ P) (◊ Q) (◊ (P ∧ ◊ Q) ∨ ◊ (◊ P ∧ Q)) | 0.
-  Proof. rewrite /CombineSepAs. apply ltl_eventually_and_r. Qed.
-
-  Class ltl_until_equiv (P Q R : tProp) :=
-    ltl_until_conv : P ≡ (Q ∪ R)%I.
-
-  Global Instance ltl_until_equiv_refl (P Q : tProp) :
-    ltl_until_equiv (P ∪ Q) P Q | 0.
-  Proof. done. Qed.
-
-  Global Instance ltl_until_equiv_next (P Q R : tProp) :
-    ltl_until_equiv P Q R →
-    ltl_until_equiv (○ P) (○ Q) (○ R) | 2.
-  Proof.
-    intros. rewrite /ltl_until_equiv. rewrite ltl_until_next_comm. by rewrite H.
-  Qed.
-
-  Global Instance ltl_eventually_equiv_next' (P Q : tProp) :
-    ltl_until_equiv P True Q →
-    ltl_until_equiv (○ P) True (○ Q) | 1.
-  Proof.
-    intros. rewrite /ltl_until_equiv.
-    rewrite ltl_eventually_next_comm. rewrite H. done.
-  Qed.
-
-  Lemma envs_clear_delete_spatial_eq {PROP} i b (Δ : envs PROP) :
-    envs_clear_spatial (envs_delete false i b Δ) = envs_clear_spatial Δ.
-  Proof.
-    destruct b.
-    - by rewrite envs_delete_intuitionistic.
-    - by destruct Δ.
-  Qed.
-
-  Global Instance elim_modal_until p P P' Q R R' :
-    ltl_until_equiv P Q R →
-    ltl_until_equiv P' Q R' →
-    ElimModal True p false modality_persistently P' R' P P.
-  Proof.
-    intros HP HP'.
-    rewrite /ElimModal.
-    iIntros "_ [HP' HP]".
-    destruct p; simpl.
-    - rewrite HP HP'.
-      iDestruct "HP'" as "#HP'".
-      iDestruct "HP" as "#HP".
-      iEval (rewrite -ltl_until_idemp).
-      by iApply (ltl_until_mono_strong Q Q R'); [eauto| |done].
-    - rewrite HP HP'.
-      iDestruct "HP" as "#HP".
-      iEval (rewrite -ltl_until_idemp).
-      by iApply (ltl_until_mono_strong Q Q R'); [eauto| |done].
-  Qed.
-
-  Global Instance from_exist_until {A} P Q (Φ : A → tProp) :
-    FromExist Q Φ → Inhabited A → FromExist (P ∪ Q) (λ a, (Φ a))%I.
-  Proof.
-    rewrite /FromExist=> HP ?. rewrite -ltl_until_intro.
-    rewrite -bi.or_intro_l. done.
-  Qed.
-
-  Lemma ltl_always_until_idemp (P Q : tProp) :
-    (□ (P ∪ Q))%I ≡ (P ∪ (□ (P ∪ Q)))%I.
-  Proof.
-    iSplit.
-    { iIntros "H". iEval (rewrite -ltl_until_intro_now). done. }
-    iApply ltl_until_ind_strong.
-    iIntros "!> [H|(HP&H&IH)]".
-    { done. }
-    rewrite -ltl_always_next_comm.
-    iDestruct "IH" as "#IH".
-    iApply ltl_always_intro.
-    { iDestruct "IH" as "#IH". iModIntro. eauto. }
-    iEval (rewrite -ltl_until_intro_next).
-    iFrame. done.
-  Qed.
-
-  (* TODO: Delete this (superfluous) lemma? *)
-  Lemma ltl_always_eventually_idemp (P : tProp) :
-    (□ ◊ P)%I ≡ (◊ □ ◊ P)%I.
-  Proof. apply ltl_always_until_idemp. Qed.
-
-  Global Instance ltl_until_equiv_always' (P Q R : tProp) :
-    ltl_until_equiv P Q R →
-    ltl_until_equiv (□ P) Q (□ P) | 1.
-  Proof.
-    intros. rewrite /ltl_until_equiv. rewrite H. apply ltl_always_until_idemp.
-  Qed.
-
-  (* TODO: Fiddle with priority order; hangs on priority 0/1 *)
-  Global Instance into_wand_until q R (P Q1 Q2 : tProp) :
-    IntoWand true false R Q1 Q2 →
-    IntoWand true q R (P ∪ Q1) (P ∪ Q2) | 10.
-  Proof.
-    rewrite /IntoWand /= => HR.
-    iIntros "#HR". destruct q.
-    - simpl. iIntros "#H". iApply (ltl_until_mono_strong with "[] [] H").
-      + eauto.
-      + iIntros "!> HQ". by iApply HR.
-    - simpl. iIntros "H". iApply (ltl_until_mono_strong with "[] [] H").
-      + eauto.
-      + iIntros "!>". by iApply HR.
-  Qed.
-
-  Lemma ltl_false_eventually :
-    ◊ False ⊢ False.
-  Proof.
-    iApply ltl_eventually_ind; [done|].
-    rewrite ltl_false_next. iDestruct 1 as "[_ $]".
-  Qed.
-
-End ltl_derived_constructs.
-
-Notation "P ∪ Q" := (ltl_until P Q%I) : bi_scope.
-Notation "◊ P" := (ltl_until True P%I) (at level 20, right associativity) : bi_scope.
-
-Tactic Notation "iModUnIntro" :=
-  iEval (rewrite -ltl_until_intro_now).
