theories/ltl_fixpoints.v
@@ -1,0 +1,531 @@
+From iris.bi Require Export fixpoint_mono.
+From iris.proofmode Require Import coq_tactics reduction spec_patterns.
+From ltl Require Export ltl.
+
+Section ltl_until.
+  Context {S L : Type}.
+  Context {Rel : S → L → S → Prop}.
+
+  Notation tProp := (tProp S L Rel).
+
+  (* Until *)
+  Definition ltl_until_F (P Q : tProp) : (() → tProp) → (() → tProp) :=
+    (λ (X : unit → tProp) _, Q ∨ (P ∧ ○ (X ())))%I.
+
+  Instance ltl_until_F_mono P Q : BiMonoPred (ltl_until_F P Q).
+  Proof.
+    constructor.
+    - intros. iIntros "#H" (x) "HF".
+      rewrite /ltl_until_F.
+      iDestruct "HF" as "[HQ|[HP HF]]"; [by iLeft|].
+      iRight. iFrame.
+      iModIntro. by iApply "H".
+    - intros. apply _.
+  Qed.
+
+  Definition ltl_until_def (P Q : tProp) : tProp :=
+    bi_least_fixpoint (ltl_until_F P Q)%I ().
+  Definition ltl_until_aux : seal (@ltl_until_def).
+  Proof. by eexists. Qed.
+  Definition ltl_until := unseal ltl_until_aux.
+  Definition ltl_until_unseal :
+    @ltl_until = @ltl_until_def := seal_eq ltl_until_aux.
+
+  Notation "P ∪ Q" := (ltl_until P Q%I) : bi_scope.
+  Notation "◊ P" := (ltl_until True P%I) (at level 20, right associativity) : bi_scope.
+
+  Lemma ltl_until_unfold (P Q : tProp) :
+    (P ∪ Q)%I ≡ (Q ∨ P ∧ ○ (P ∪ Q))%I.
+  Proof. rewrite ltl_until_unseal. by rewrite /ltl_until_def {1}least_fixpoint_unfold. Qed.
+
+  Lemma ltl_until_intro (P Q : tProp) :
+    Q ∨ P ∧ ○ (P ∪ Q) ⊢ P ∪ Q.
+  Proof. rewrite {2}ltl_until_unfold. done. Qed.
+
+  Lemma ltl_until_ind_strong (P Q R : tProp) :
+    □ (Q ∨ (P ∧ ○ (P ∪ Q) ∧ ○ R) → R) ⊢
+    P ∪ Q → R.
+  Proof.
+    iIntros "#IH HPQ".
+    rewrite ltl_until_unseal.
+    iApply (least_fixpoint_ind with "[] HPQ").
+    iIntros "!>" (?) "[Q|[HP HR]]".
+    { iApply "IH". by eauto. }
+    iApply "IH". iRight. iFrame.
+    iSplit.
+    - iModIntro. iDestruct "HR" as "[_ $]".
+    - iModIntro. iDestruct "HR" as "[$ _]".
+  Qed.
+
+  Lemma ltl_until_ind (P Q R : tProp) :
+    (Q ∨ (P ∧ ○ (P ∪ Q) ∧ ○ R) ⊢ R) →
+    (P ∪ Q ⊢ R).
+  Proof.
+    intros IH.
+    iApply ltl_until_ind_strong. iIntros "!> H". iApply IH. done.
+  Qed.
+
+  Lemma ltl_until_intro_now (P Q : tProp) :
+    Q ⊢ P ∪ Q.
+  Proof. rewrite -ltl_until_intro. apply bi.or_intro_l. Qed.
+
+  Lemma ltl_until_intro_next (P Q : tProp) :
+    P ∧ ○ (P ∪ Q) ⊢ P ∪ Q.
+  Proof. rewrite -{2}ltl_until_intro. apply bi.or_intro_r. Qed.
+
+  Lemma ltl_until_mono_strong P1 P2 Q1 Q2 :
+    □ (P1 → P2) ⊢ □ (Q1 → Q2) →
+    P1 ∪ Q1 → P2 ∪ Q2.
+  Proof.
+    iIntros "#HP #HQ HPQ".
+    iApply (ltl_until_ind_strong with "[] HPQ").
+    iModIntro.
+    iDestruct 1 as "[H|H]".
+    { rewrite ltl_until_unfold. iLeft. by iApply "HQ". }
+    iEval (rewrite ltl_until_unfold). iRight.
+    iDestruct "H" as "[H IH]".
+    iSplit.
+    - by iApply "HP".
+    - iDestruct "IH" as "[_ $]".
+  Qed.
+
+  Lemma ltl_until_mono P1 P2 Q1 Q2 :
+    (P1 ⊢ P2) → (Q1 ⊢ Q2) →
+    P1 ∪ Q1 ⊢ P2 ∪ Q2.
+  Proof.
+    intros HP HQ.
+    iApply ltl_until_mono_strong.
+    iApply HP.
+    iApply HQ.
+  Qed.
+
+  Lemma ltl_until_and (P Q1 Q2 : tProp) :
+    (P ∪ (Q1 ∧ Q2)) ⊢ (P ∪ Q1) ∧ (P ∪ Q2).
+  Proof.
+    rewrite ltl_until_unfold.
+    iIntros "[H|H]".
+    { iDestruct "H" as "[H1 H2]".
+      rewrite (ltl_until_unfold _ Q1).
+      rewrite (ltl_until_unfold _ Q2).
+      iSplit; by iLeft. }
+    iSplit.
+    - iEval (rewrite ltl_until_unfold).
+      iRight. iDestruct "H" as "[$ H]".
+      iModIntro. iApply (ltl_until_mono_strong with "[] [] H").
+      + eauto.
+      + iIntros "!>[$ _]".
+    - iEval (rewrite ltl_until_unfold).
+      iRight. iDestruct "H" as "[$ H]".
+      iModIntro. iApply (ltl_until_mono_strong with "[] [] H").
+      + eauto.
+      + iIntros "!>[_ $]".
+  Qed.
+
+  Lemma ltl_until_always_combine (P Q R : tProp) :
+    (□ P ∧ Q ∪ R) ⊢ (((Q ∧ □ P) ∪ (R ∧ □ P))).
+  Proof.
+    iIntros "[#HP HQ]".
+    iApply (ltl_until_ind_strong with "[] HQ").
+    iIntros "!> [HQ|H]".
+    { iApply ltl_until_intro_now. iFrame "#∗". }
+    iEval (rewrite -ltl_until_intro_next).
+    iDestruct "H" as "[$ H]".
+    iSplit; [done|].
+    iModIntro.
+    iDestruct "H" as "[_ $]".
+  Qed.
+
+  Lemma ltl_until_next_comm (P Q : tProp) :
+    (○ P ∪ ○ Q) ⊣⊢ ○ (P ∪ Q).
+  Proof.
+    iSplit.
+    - iApply ltl_until_ind_strong.
+      iIntros "!>H".
+      iDestruct "H" as "[HQ|H]".
+      + iModIntro. rewrite ltl_until_unfold. by iLeft.
+      + iModIntro. iEval (rewrite ltl_until_unfold). iRight.
+        iDestruct "H" as "[$ [HP HQ]]". iModIntro. done.
+    - iIntros "H".
+      iEval (rewrite ltl_until_unfold).
+      rewrite ltl_next_and.
+      iEval (rewrite (ltl_next_or Q)).
+      iModIntro.
+      iApply (ltl_until_ind_strong with "[] H").
+      iIntros "!>H".
+      iDestruct "H" as "[H|H]".
+      { iLeft. done. }
+      iRight.
+      iDestruct "H" as "[$ [_ H]]".
+      rewrite {2}ltl_until_unfold.
+      rewrite ltl_next_and ltl_next_or.
+      iModIntro.
+      iDestruct "H" as "[H|H]".
+      { iLeft. done. }
+      iRight.
+      done.
+  Qed.
+
+  Lemma ltl_until_idemp (P Q : tProp) :
+    (P ∪ (P ∪ Q)) ⊣⊢ (P ∪ Q).
+  Proof.
+    iSplit.
+    - iApply ltl_until_ind_strong.
+      iIntros "!> [H|(?&?&?)]".
+      { done. }
+      iEval (rewrite ltl_until_unfold). iRight. iFrame.
+    - iApply ltl_until_ind_strong.
+      iIntros "!> [H|(?&?&?)]".
+      { rewrite ltl_until_unfold. iLeft. rewrite ltl_until_unfold. iLeft. done. }
+      iEval (rewrite ltl_until_unfold). iRight. iFrame.
+  Qed.
+
+  Lemma ltl_until_and_r' (P1 P2 Q1 Q2 : tProp) :
+    P1 ∪ Q1 ∧ P2 ∪ Q2 ⊢ (P1 ∧ P2) ∪ ((Q1 ∧ P2 ∪ Q2) ∨ (P1 ∪ Q1 ∧ Q2)).
+  Proof.
+    iIntros "[H1 H2]".
+    iRevert "H2".
+    iApply (ltl_until_ind_strong with "[] H1").
+    iIntros "!> H1 H2".
+    rewrite {3}(ltl_until_unfold P2 Q2).
+    iDestruct "H1" as "[HQ1|(HP1&HPQ1&IH)]".
+    { iDestruct "H2" as "[HQ2|[HP2 HPQ2]]".
+      { iEval (rewrite ltl_until_unfold). iLeft.
+        iEval (rewrite ltl_until_unfold). iFrame. }
+      { iEval (rewrite ltl_until_unfold). iLeft. iLeft. iFrame.
+        iEval (rewrite ltl_until_unfold). iRight. iFrame. }
+    }
+    iDestruct "H2" as "[HQ2|[HP2 HPQ2]]".
+    { iEval (rewrite ltl_until_unfold). iLeft.
+      iEval (rewrite ltl_until_unfold). iRight.
+      iEval (rewrite ltl_until_unfold). iFrame. iRight. iFrame. }
+    iEval (rewrite ltl_until_unfold). iRight.
+    iFrame. iModIntro.
+    by iApply "IH".
+  Qed.
+
+  Lemma ltl_until_or (P Q1 Q2 : tProp) :
+    P ∪ (Q1 ∨ Q2) ⊢ P ∪ Q1 ∨ P ∪ Q2.
+  Proof.
+    iApply ltl_until_ind_strong.
+    iIntros "!> [HQ|HP]".
+    { iDestruct "HQ" as "[HQ1|HQ2]".
+      - iLeft. by rewrite -ltl_until_intro_now.
+      - iRight. by rewrite -ltl_until_intro_now.
+    }
+    iDestruct "HP" as "(HP&HPQ&IH)".
+    rewrite -!ltl_until_next_comm.
+    rewrite {1}(ltl_next_or_2 (P ∪ Q1)).
+    iDestruct "IH" as "[IH|IH]".
+    - iLeft. iEval (rewrite ltl_until_unfold).
+      iRight. iFrame.
+    - iRight. iEval (rewrite ltl_until_unfold).
+      iRight. iFrame.
+  Qed.
+
+  Lemma ltl_until_and_r (P1 P2 Q1 Q2 : tProp) :
+    P1 ∪ Q1 ∧ P2 ∪ Q2 ⊢ ((P1 ∧ P2) ∪ (Q1 ∧ (P2 ∪ Q2))) ∨ ((P1 ∧ P2) ∪ (P1 ∪ Q1 ∧ Q2)).
+  Proof. rewrite -ltl_until_or. apply ltl_until_and_r'. Qed.
+
+  Global Instance ltl_until_proper : Proper ((≡) ==> (≡) ==> (≡)) (ltl_until).
+  Proof.
+    constructor.
+    intros. split.
+    - apply ltl_until_mono; [by rewrite H|by rewrite H0].
+    - apply ltl_until_mono; [by rewrite H|by rewrite H0].
+  Qed.
+  Global Instance ltl_until_mono' :
+    Proper ((⊢) ==> (⊢) ==> (⊢)) (ltl_until).
+  Proof.
+    constructor.
+    intros ?. apply ltl_until_mono; [by rewrite H|by rewrite H0].
+  Qed.
+  Global Instance ltl_until_flip_mono' :
+    Proper (flip (⊢) ==> flip (⊢) ==> flip (⊢)) (ltl_until).
+  Proof.
+    constructor.
+    intros ?. apply ltl_until_mono; [by rewrite H|by rewrite H0].
+  Qed.
+
+  Global Instance ltl_until_combine (P1 P2 Q1 Q2 : tProp) :
+    CombineSepAs (P1 ∪ Q1) (P2 ∪ Q2)
+      (((P1 ∧ P2) ∪ (Q1 ∧ (P2 ∪ Q2))) ∨ ((P1 ∧ P2) ∪ (P1 ∪ Q1 ∧ Q2))) | 1.
+  Proof. rewrite /CombineSepAs. apply ltl_until_and_r. Qed.
+
+  Lemma ltl_eventually_intro (P : tProp) :
+    P ∨ ○ ◊ P ⊢ ◊ P.
+  Proof.
+    rewrite -{2}(ltl_until_intro True P).
+    iIntros "[HP|HP]".
+    { by iLeft. }
+    iRight. by iFrame.
+  Qed.
+
+  Lemma ltl_eventually_intro_now (P : tProp) :
+    P ⊢ ◊ P.
+  Proof. rewrite -ltl_until_intro. apply bi.or_intro_l. Qed.
+
+  Lemma ltl_eventually_intro_next (P : tProp) :
+    (○ P) ⊢ (◊ P).
+  Proof. rewrite -ltl_eventually_intro.
+         etrans; [|apply bi.or_intro_r]. apply ltl_next_mono.
+         apply ltl_eventually_intro_now.
+  Qed.
+
+  Lemma ltl_eventually_mono_strong (P Q : tProp) :
+    □ (P → Q) ⊢ ◊P → ◊Q.
+  Proof. by iApply ltl_until_mono_strong. Qed.
+
+  Lemma ltl_eventually_mono (P Q : tProp) :
+    (P ⊢ Q) → (◊P) ⊢ (◊Q).
+  Proof. by apply ltl_until_mono. Qed.
+
+  Lemma ltl_eventually_and (P Q : tProp) :
+    (◊ (P ∧ Q)) ⊢ (◊ P) ∧ (◊ Q).
+  Proof. by rewrite -ltl_until_and. Qed.
+
+  Lemma ltl_eventually_next_comm (P : tProp) :
+    (◊ ○ P) ⊣⊢ (○ ◊ P).
+  Proof.
+    rewrite -ltl_until_next_comm.
+    apply bi.equiv_entails_2.
+    - apply ltl_until_mono; [|done]. by apply ltl_next_emp.
+    - apply ltl_until_mono; [|done]. eauto.
+  Qed.
+
+  Lemma ltl_eventually_idemp (P : tProp) :
+    (◊◊P) ⊣⊢ (◊P).
+  Proof. apply ltl_until_idemp. Qed.
+
+  Lemma ltl_eventually_next (P : tProp) :
+    (◊ ○ P) ⊢ (◊ P).
+  Proof.
+    rewrite <-(ltl_eventually_idemp P).
+    apply ltl_eventually_mono.
+    apply ltl_eventually_intro_next.
+  Qed.
+
+  Lemma ltl_next_eventually (P : tProp) :
+    (○ ◊ P) ⊢ (◊ P).
+  Proof. rewrite -{2}ltl_eventually_next ltl_eventually_next_comm. done. Qed.
+
+  Lemma ltl_until_eventually_equiv (P : tProp) :
+    (True ∪ P) ⊣⊢ (◊ P).
+  Proof. done. Qed.
+
+  Lemma ltl_until_eventually (P Q : tProp) :
+    (P ∪ Q) ⊢ (◊ Q).
+  Proof. apply ltl_until_mono; by eauto. Qed.
+
+  Lemma ltl_eventually_ind_strong (P Q : tProp) :
+    (□ (P ∨ ○ ◊ P ∧ ○ Q → Q)) ⊢ ◊ P → Q.
+  Proof.
+    iIntros "#H". iApply ltl_until_ind_strong.
+    iModIntro. iIntros "[HP|HP]".
+    { iApply "H". iLeft. done. }
+    iApply "H". iRight. iDestruct "HP" as "[_ $]".
+  Qed.
+
+  Lemma ltl_eventually_ind (P Q : tProp) :
+    (P ⊢ Q) →
+    ((○ ◊ P) ∧ ○ Q ⊢ Q) →
+    ◊ P ⊢ Q.
+  Proof.
+    intros H1 H2.
+    iApply ltl_eventually_ind_strong.
+    iDestruct H1 as "#H1".
+    iDestruct H2 as "#H2".
+    iModIntro. iIntros "[HP|HP]"; [by iApply "H1"|by iApply "H2"].
+  Qed.
+
+  Lemma ltl_always_eventually (P : tProp) :
+    □ P ⊢ ◊ P.
+  Proof. rewrite -ltl_eventually_intro_now. eauto. Qed.
+
+  Lemma ltl_eventually_always_combine (P Q : tProp) :
+    (□ P ∧ ◊Q) ⊢ (◊ (Q ∧ □ P)).
+  Proof.
+    iIntros "[#HP HQ]".
+    iApply (ltl_eventually_ind_strong with "[] HQ").
+    iIntros "!> [HQ|H]".
+    { iApply ltl_eventually_intro_now. iFrame "#∗". }
+    iEval (rewrite -ltl_eventually_idemp).
+    iEval (rewrite -ltl_eventually_intro_next).
+    iModIntro.
+    iDestruct "H" as "[_ $]".
+  Qed.
+
+  Lemma ltl_not_eventually_always_not (P : tProp) :
+    ¬ ◊ P ⊢ □ (¬ P).
+  Proof.
+    iIntros "H".
+    iAssert (□ ((¬ ◊ P) ∧ (¬ P)))%I with "[H]" as "#[H1 H2]"; last first.
+    { iApply ltl_always_intro; last first.
+      { done. }
+      iIntros "!> H !>". iFrame "#". }
+    iApply ltl_always_intro; last first.
+    { iSplit.
+      - done.
+      - iIntros "HP". iApply "H". rewrite -ltl_eventually_intro_now. done. }
+    iIntros "!> [H1 H2]".
+    rewrite -ltl_next_and.
+    iSplit.
+    - rewrite -ltl_next_not. iIntros "H". iApply "H1". rewrite ltl_next_eventually. done.
+    - rewrite -ltl_next_not. iIntros "H". iApply "H1". rewrite -ltl_next_eventually. iModIntro. rewrite -ltl_eventually_intro_now. done.
+  Qed.
+
+  Global Instance into_and_eventually (P Q1 Q2 : tProp) :
+    IntoAnd false P Q1 Q2 →
+    IntoAnd false (◊ P)%I (◊ Q1)%I (◊ Q2)%I.
+  Proof.
+    rewrite /IntoAnd. simpl.
+    intros HPQ.
+    rewrite -ltl_eventually_and.
+    by eapply ltl_eventually_mono.
+  Qed.
+
+  Global Instance into_sep_eventually (P Q1 Q2 : tProp) :
+    IntoSep P Q1 Q2 →
+    IntoSep (◊ P)%I (◊ Q1)%I (◊ Q2)%I.
+  Proof.
+    rewrite /IntoSep.
+    simpl.
+    rewrite !bi_sep_and.
+    intros HPQ.
+    rewrite -ltl_eventually_and.
+    by eapply ltl_eventually_mono.
+  Qed.
+
+  Global Instance into_next_eventually (P Q : tProp) :
+    IntoNext false P Q →
+    IntoNext false (◊ P) (◊ Q).
+  Proof.
+    rewrite /IntoNext. intros HPQ.
+    rewrite -ltl_eventually_next_comm.
+    eapply ltl_eventually_mono.
+    specialize HPQ. simpl in HPQ.
+    done.
+  Qed.
+
+  Lemma ltl_eventually_and_r (P Q : tProp) :
+    ◊ P ∧ ◊ Q ⊢ ◊ (P ∧ ◊ Q) ∨ ◊ (◊ P ∧ Q).
+  Proof. by rewrite ltl_until_and_r right_id. Qed.
+
+  Global Instance ltl_eventually_combine (P Q : tProp) :
+    CombineSepAs (◊ P) (◊ Q) (◊ (P ∧ ◊ Q) ∨ ◊ (◊ P ∧ Q)) | 0.
+  Proof. rewrite /CombineSepAs. apply ltl_eventually_and_r. Qed.
+
+  Class ltl_until_equiv (P Q R : tProp) :=
+    ltl_until_conv : P ≡ (Q ∪ R)%I.
+
+  Global Instance ltl_until_equiv_refl (P Q : tProp) :
+    ltl_until_equiv (P ∪ Q) P Q | 0.
+  Proof. done. Qed.
+
+  Global Instance ltl_until_equiv_next (P Q R : tProp) :
+    ltl_until_equiv P Q R →
+    ltl_until_equiv (○ P) (○ Q) (○ R) | 2.
+  Proof.
+    intros. rewrite /ltl_until_equiv. rewrite ltl_until_next_comm. by rewrite H.
+  Qed.
+
+  Global Instance ltl_eventually_equiv_next' (P Q : tProp) :
+    ltl_until_equiv P True Q →
+    ltl_until_equiv (○ P) True (○ Q) | 1.
+  Proof.
+    intros. rewrite /ltl_until_equiv.
+    rewrite ltl_eventually_next_comm. rewrite H. done.
+  Qed.
+
+  Lemma envs_clear_delete_spatial_eq {PROP} i b (Δ : envs PROP) :
+    envs_clear_spatial (envs_delete false i b Δ) = envs_clear_spatial Δ.
+  Proof.
+    destruct b.
+    - by rewrite envs_delete_intuitionistic.
+    - by destruct Δ.
+  Qed.
+
+  Global Instance elim_modal_until p P P' Q R R' :
+    ltl_until_equiv P Q R →
+    ltl_until_equiv P' Q R' →
+    ElimModal True p false modality_persistently P' R' P P.
+  Proof.
+    intros HP HP'.
+    rewrite /ElimModal.
+    iIntros "_ [HP' HP]".
+    destruct p; simpl.
+    - rewrite HP HP'.
+      iDestruct "HP'" as "#HP'".
+      iDestruct "HP" as "#HP".
+      iEval (rewrite -ltl_until_idemp).
+      by iApply (ltl_until_mono_strong Q Q R'); [eauto| |done].
+    - rewrite HP HP'.
+      iDestruct "HP" as "#HP".
+      iEval (rewrite -ltl_until_idemp).
+      by iApply (ltl_until_mono_strong Q Q R'); [eauto| |done].
+  Qed.
+
+  Global Instance from_exist_until {A} P Q (Φ : A → tProp) :
+    FromExist Q Φ → Inhabited A → FromExist (P ∪ Q) (λ a, (Φ a))%I.
+  Proof.
+    rewrite /FromExist=> HP ?. rewrite -ltl_until_intro.
+    rewrite -bi.or_intro_l. done.
+  Qed.
+
+  Lemma ltl_always_until_idemp (P Q : tProp) :
+    (□ (P ∪ Q))%I ≡ (P ∪ (□ (P ∪ Q)))%I.
+  Proof.
+    iSplit.
+    { iIntros "H". iEval (rewrite -ltl_until_intro_now). done. }
+    iApply ltl_until_ind_strong.
+    iIntros "!> [H|(HP&H&IH)]".
+    { done. }
+    rewrite -ltl_always_next_comm.
+    iDestruct "IH" as "#IH".
+    iApply ltl_always_intro.
+    { iDestruct "IH" as "#IH". iModIntro. eauto. }
+    iEval (rewrite -ltl_until_intro_next).
+    iFrame. done.
+  Qed.
+
+  (* TODO: Delete this (superfluous) lemma? *)
+  Lemma ltl_always_eventually_idemp (P : tProp) :
+    (□ ◊ P)%I ≡ (◊ □ ◊ P)%I.
+  Proof. apply ltl_always_until_idemp. Qed.
+
+  Global Instance ltl_until_equiv_always' (P Q R : tProp) :
+    ltl_until_equiv P Q R →
+    ltl_until_equiv (□ P) Q (□ P) | 1.
+  Proof.
+    intros. rewrite /ltl_until_equiv. rewrite H. apply ltl_always_until_idemp.
+  Qed.
+
+  (* TODO: Fiddle with priority order; hangs on priority 0/1 *)
+  Global Instance into_wand_until q R (P Q1 Q2 : tProp) :
+    IntoWand true false R Q1 Q2 →
+    IntoWand true q R (P ∪ Q1) (P ∪ Q2) | 10.
+  Proof.
+    rewrite /IntoWand /= => HR.
+    iIntros "#HR". destruct q.
+    - simpl. iIntros "#H". iApply (ltl_until_mono_strong with "[] [] H").
+      + eauto.
+      + iIntros "!> HQ". by iApply HR.
+    - simpl. iIntros "H". iApply (ltl_until_mono_strong with "[] [] H").
+      + eauto.
+      + iIntros "!>". by iApply HR.
+  Qed.
+
+  Lemma ltl_false_eventually :
+    ◊ False ⊢ False.
+  Proof.
+    iApply ltl_eventually_ind; [done|].
+    rewrite ltl_false_next. iDestruct 1 as "[_ $]".
+  Qed.
+
+  Global Instance from_modal_until (P Q : tProp) :
+    @FromModal ltlI ltlI _ True%type modality_id (P ∪ Q) (P ∪ Q) (Q).
+  Proof. intros _. apply ltl_until_intro_now. Qed.
+
+End ltl_until.
+
+Global Notation "P ∪ Q" := (ltl_until P Q%I) : bi_scope.
+Global Notation "◊ P" := (ltl_until True P%I) (at level 20, right associativity) : bi_scope.
