theories/trace.v
@@ -1,0 +1,68 @@
+From stdpp Require Import option.
+
+Delimit Scope trace_scope with trace.
+
+CoInductive trace_aux (S L : Type) :=
+| tr_singl (s: S)
+| tr_cons (s: S) (ℓ: L) (r: trace_aux S L).
+
+Definition trace (S L : Type) := option $ trace_aux S L.
+
+Arguments tr_singl {_} {_} _.
+Arguments tr_cons {_} {_} _ _ _.
+
+Bind Scope trace_scope with trace.
+
+Arguments tr_singl {_} {_} _.
+Arguments tr_cons {_} {_} _ _ _%trace.
+Notation "⟨ ⟩" := (None) : trace_scope.
+Notation "⟨ s ⟩" := (Some (tr_singl s)) : trace_scope.
+Notation "s -[ ℓ ]->  r" := (Some (tr_cons s ℓ r)) (at level 33) : trace_scope.
+Open Scope trace.
+
+Section well_formed.
+  Context {S L : Type}.
+  Context (R : S → L → S → Prop).
+
+  Definition head_trace' (tr : trace_aux S L) : S * option L :=
+    match tr with
+    | tr_singl s => (s, None)
+    | tr_cons s ℓ tr => (s, Some ℓ)
+    end.
+
+  Definition head_trace : trace S L → option (S * option L) :=
+    fmap head_trace'.
+
+  Definition tail_trace' (tr : trace_aux S L) : option (trace_aux S L) :=
+    match tr with
+    | tr_singl s => None
+    | tr_cons s ℓ r => Some r
+    end.
+
+  Definition tail_trace : trace S L → trace S L :=
+    mbind tail_trace'.
+
+  CoInductive trace_maximal : trace S L → SProp :=
+  | trace_maximal_empty : trace_maximal None
+  | trace_maximal_singleton c :
+    (∀ oζ c', ¬ R c oζ c') → trace_maximal (Some $ tr_singl c)
+  | trace_maximal_cons c l tr c' :
+    fst <$> head_trace (Some tr) = Some c' →
+    R c l c' →
+    trace_maximal (Some tr) →
+    trace_maximal (Some $ tr_cons c l tr).
+
+End well_formed.
+
+Record wf_trace S L R := Trace {
+  tr_car : trace S L;
+  tr_wf : trace_maximal R tr_car;
+}.
+
+Arguments Trace {_ _ _} _ _.
+Arguments tr_car {_ _ _} _.
+Arguments tr_wf {_ _ _} _.
+Arguments trace_maximal_empty {_ _ _}.
+Arguments trace_maximal_singleton {_ _ _} _ _.
+
+Notation "tr @ tr_wf" := (Trace tr tr_wf) (at level 100).
